src/ldrfra/PFtoAPFSimThread.v
@@ -1,0 +1,75 @@
+Require Import Omega.
+Require Import Bool.
+Require Import RelationClasses.
+
+From sflib Require Import sflib.
+From Paco Require Import paco.
+
+From PromisingLib Require Import Axioms.
+From PromisingLib Require Import Basic.
+From PromisingLib Require Import DataStructure.
+From PromisingLib Require Import DenseOrder.
+From PromisingLib Require Import Loc.
+From PromisingLib Require Import Language.
+
+Require Import Event.
+Require Import Time.
+Require Import View.
+Require Import Cell.
+Require Import Memory.
+Require Import TView.
+Require Import Local.
+Require Import Thread.
+
+Require Import MemoryMerge.
+
+Require Import PFStep.
+Require Import OrdStep.
+Require Import RelWrites.
+Require Import RelStep.
+
+Set Implicit Arguments.
+
+
+Module PFtoAPFSimThread.
+  Section PFtoAPFSimThread.
+    Variable lang: language.
+    Variable L: Loc.t -> bool.
+
+    Variant sim_memory (rels: RelWrites.t) (mem_src mem_tgt: Memory.t): Prop :=
+    | sim_memory_intro
+        (SOUND: Memory.le mem_src mem_tgt)
+        (COMPLETE1: forall loc (LOC: L loc), Cell.le (mem_tgt loc) (mem_src loc))
+        (COMPLETE2: forall loc ts from to msg
+                      (LOC: ~ L loc) (LE: Time.le ts to)
+                      (GET_TGT: Memory.get loc to mem_tgt = Some (from, msg)),
+            (<<GET_SRC: Memory.get loc to mem_src = Some (from, msg)>>) \/
+            exists from' to' val released,
+              (<<LT: Time.lt ts to'>>) /\
+              (<<GET_SRC: Memory.get loc to' mem_src = Some (from', Message.concrete val released)>>))
+        (RESERVE: forall loc from to
+                    (GET_TGT: Memory.get loc to mem_tgt = Some (from, Message.reserve)),
+            (<<GET_SRC: Memory.get loc to mem_src = Some (from, Message.reserve)>>))
+    .
+    Hint Constructors sim_memory.
+
+    Inductive sim_statelocal (rels: RelWrites.t):
+      forall (sl_src sl_tgt: {lang : language & Language.state lang} * Local.t), Prop :=
+    | sim_statelocal_intro
+        lang st lc_src lc_tgt
+        (LOCAL: lc_src = lc_tgt):
+        sim_statelocal rels (existT _ lang st, lc_src) (existT _ lang st, lc_tgt)
+    .
+    Hint Constructors sim_statelocal.
+
+    Inductive sim_thread (rels: RelWrites.t) (e_src e_tgt: Thread.t lang): Prop :=
+    | sim_thread_intro
+        (STATE: (Thread.state e_src) = (Thread.state e_tgt))
+        (LOCAL: (Thread.local e_src) = (Thread.local e_tgt))
+        (PROMISES: OrdLocal.reserve_only L (Local.promises (Thread.local e_src)))
+        (SC: (Thread.sc e_src) = (Thread.sc e_tgt))
+        (MEMORY: sim_memory rels (Thread.memory e_src) (Thread.memory e_tgt))
+    .
+    Hint Constructors sim_thread.
+  End PFtoAPFSimThread.
+End PFtoAPFSimThread.
