src/ldrfra/RelWrites.v
@@ -20,6 +20,9 @@ Require Import Memory.
 Require Import MemoryFacts.
 Require Import TView.
 Require Import Local.
+Require Import Thread.
+
+Require Import OrdStep.
 
 Set Implicit Arguments.
 
@@ -43,12 +46,180 @@ Module RelWrites.
       forall loc to (IN: List.In (loc, to) rels),
         Memory.get loc to promises = None /\
         exists from val released,
-          Memory.get loc to mem = Some (from, Message.concrete val released).
+          Memory.get loc to mem = Some (from, Message.concrete val (Some released)).
 
     Lemma append_app e rels1 rels2:
       append e rels1 ++ rels2 = append e (rels1 ++ rels2).
     Proof.
       unfold append. des_ifs.
+    Qed.
+
+    Lemma promise_wf
+          rels promises1 mem1 loc from to msg promises2 mem2 kind
+          (RELS1: wf rels promises1 mem1)
+          (PROMISE: Memory.promise promises1 mem1 loc from to msg promises2 mem2 kind):
+      wf rels promises2 mem2.
+    Proof.
+      ii. exploit RELS1; eauto. i. des. inv PROMISE; ss.
+      - exploit Memory.add_get1; try exact x0; eauto. i. esplits; eauto.
+        erewrite Memory.add_o; eauto. condtac; ss. des. subst.
+        exploit Memory.add_get0; try exact MEM. i. des. congr.
+      - exploit Memory.split_get1; try exact x0; eauto. i. des. subst. esplits; eauto.
+        erewrite Memory.split_o; eauto. repeat condtac; ss.
+        + des. subst. exploit Memory.split_get0; try exact MEM. i. des. congr.
+        + guardH o. des. subst.
+          exploit Memory.split_get0; try exact PROMISES. i. des. congr.
+      - exploit Memory.lower_get1; try exact x0; eauto. i. des. inv MSG_LE.
+        dup GET2. revert GET2. erewrite Memory.lower_o; eauto. condtac; ss.
+        + i. des. inv GET2.
+          exploit Memory.lower_get0; try exact PROMISES. i. des. congr.
+        + guardH o. i. rewrite GET2 in *. inv x0. esplits; eauto.
+          erewrite Memory.lower_o; eauto. condtac; ss.
+      - erewrite (@Memory.remove_o promises2); eauto.
+        erewrite (@Memory.remove_o mem2); eauto. condtac; ss; eauto.
+        des. subst. exploit Memory.remove_get0; try exact PROMISES. i. des. congr.
+    Qed.
+
+    Lemma write_wf
+          rels promises1 mem1 loc from to msg promises2 mem2 kind
+          (RELS1: wf rels promises1 mem1)
+          (WRITE: Memory.write promises1 mem1 loc from to msg promises2 mem2 kind):
+      wf rels promises2 mem2.
+    Proof.
+      inv WRITE. hexploit promise_wf; eauto. i.
+      ii. exploit H; eauto. i. des. esplits; eauto.
+      erewrite Memory.remove_o; eauto. condtac; ss.
+    Qed.
+
+    Lemma write_wf_incr
+          rels promises1 mem1 loc from to msg promises2 mem2 kind
+          (RELS1: wf rels promises1 mem1)
+          (WRITE: Memory.write promises1 mem1 loc from to msg promises2 mem2 kind)
+          (MSG: exists val released, msg = Message.concrete val (Some released)):
+      wf ((loc, to)::rels) promises2 mem2.
+    Proof.
+      des. hexploit write_wf; eauto. ii.
+      inv IN; eauto. inv H0.
+      exploit Memory.write_not_cancel; eauto. i.
+      inv WRITE. exploit Memory.promise_get0; eauto. i. des.
+      exploit Memory.remove_get0; eauto. i. des.
+      esplits; eauto.
+    Qed.
+
+    Lemma write_na_wf
+          rels ts promises1 mem1 loc from to msg promises2 mem2 msgs kinds kind
+          (RELS1: wf rels promises1 mem1)
+          (WRITE: Memory.write_na ts promises1 mem1 loc from to msg promises2 mem2 msgs kinds kind):
+      wf rels promises2 mem2.
+    Proof.
+      induction WRITE; eauto using write_wf.
+    Qed.
+
+    Lemma step_wf
+          ordcr ordcw rels lang pf e e1 e2
+          (RELS1: wf rels (Local.promises (Thread.local e1)) (Thread.memory e1))
+          (STEP: @OrdThread.step lang L ordcr ordcw pf e e1 e2):
+      wf (append e rels) (Local.promises (Thread.local e2)) (Thread.memory e2).
+    Proof.
+      unfold append.
+      inv STEP; inv STEP0; inv LOCAL; try inv LOCAL0; ss.
+      - eapply promise_wf; eauto.
+      - inv STEP. ss.
+      - inv STEP. hexploit write_wf; eauto. i.
+        repeat condtac; eauto.
+        revert WRITE. unfold TView.write_released.
+        condtac; try by destruct ord, ordcw; ss. i.
+        hexploit write_wf_incr; try exact WRITE; eauto.
+      - inv LOCAL1. inv STEP. inv LOCAL2. inv STEP. ss.
+        hexploit write_wf; eauto. i.
+        repeat condtac; eauto.
+        revert WRITE. unfold TView.write_released.
+        condtac; try by destruct ordw, ordcw; ss. i.
+        hexploit write_wf_incr; try exact WRITE; eauto.
+      - inv STEP. hexploit write_na_wf; eauto. i.
+        repeat condtac; eauto.
+        destruct ord, ordcw; ss.
+    Qed.
+
+    Lemma promise_disjoint
+          promises1 mem1 loc from to msg promises2 mem2 kind
+          promises
+          (PROMISE: Memory.promise promises1 mem1 loc from to msg promises2 mem2 kind)
+          (DISJOINT: Memory.disjoint promises1 promises)
+          (LE: Memory.le promises mem1):
+      Memory.get loc to promises = None.
+    Proof.
+      destruct (Memory.get loc to promises) as [[]|] eqn:GETP; ss.
+      exploit LE; eauto. i.
+      inv PROMISE; ss.
+      - exploit Memory.add_get0; try exact MEM. i. des. congr.
+      - exploit Memory.split_get0; try exact MEM. i. des. congr.
+      - exploit Memory.lower_get0; try exact PROMISES. i. des.
+        inv DISJOINT. exploit DISJOINT0; eauto. i. des. exfalso.
+        exploit Memory.get_ts; try exact GETP. i. des; try congr.
+        exploit Memory.get_ts; try exact GET. i. des; try congr.
+        apply (x0 to); econs; try refl; ss.
+      - exploit Memory.remove_get0; try exact PROMISES. i. des.
+        inv DISJOINT. exploit DISJOINT0; eauto. i. des. exfalso.
+        exploit Memory.get_ts; try exact GETP. i. des; try congr.
+        exploit Memory.get_ts; try exact GET. i. des; try congr.
+        apply (x0 to); econs; try refl; ss.
+    Qed.
+
+    Lemma write_disjoint
+          promises1 mem1 loc from to msg promises2 mem2 kind
+          promises
+          (WRITE: Memory.write promises1 mem1 loc from to msg promises2 mem2 kind)
+          (DISJOINT: Memory.disjoint promises1 promises)
+          (LE: Memory.le promises mem1):
+      Memory.get loc to promises = None.
+    Proof.
+      inv WRITE. eauto using promise_disjoint.
+    Qed.
+
+    Lemma write_na_disjoint
+          ts promises1 mem1 loc from to msg promises2 mem2 msgs kinds kind
+          promises
+          (WRITE: Memory.write_na ts promises1 mem1 loc from to msg promises2 mem2 msgs kinds kind)
+          (DISJOINT: Memory.disjoint promises1 promises)
+          (LE: Memory.le promises mem1):
+      Memory.get loc to promises = None.
+    Proof.
+      induction WRITE; eauto using write_disjoint.
+      exploit Memory.write_disjoint; try exact WRITE_EX; eauto. i. des. eauto.
+    Qed.
+
+    Lemma step_disjoint
+          ordrc ordwc rels lang pf e e1 e2 promises
+          (RELS1: wf rels (Local.promises (Thread.local e1)) (Thread.memory e1))
+          (STEP: @OrdThread.step lang L ordrc ordwc pf e e1 e2)
+          (DISJOINT: Memory.disjoint (Local.promises (Thread.local e1)) promises)
+          (LE: Memory.le promises (Thread.memory e1))
+          (RELS: wf rels promises (Thread.memory e1)):
+      wf (append e rels) promises (Thread.memory e2).
+    Proof.
+      hexploit step_wf; eauto. ii.
+      exploit H; eauto. i. des. esplits; eauto.
+      unfold RelWrites.append in *.
+      inv STEP; inv STEP0; inv LOCAL; ss.
+      - exploit RELS; eauto. i. des. ss.
+      - exploit RELS; eauto. i. des. ss.
+      - exploit RELS; eauto. i. des. ss.
+      - inv LOCAL0. inv STEP. ss. revert IN.
+        repeat condtac; ss; i; des; try by (exploit RELS; eauto; i; des; ss).
+        inv IN. eapply write_disjoint; eauto.
+      - inv LOCAL1. inv STEP. inv LOCAL2. inv STEP. ss. revert IN.
+        repeat condtac; ss; i; des; try by (exploit RELS; eauto; i; des; ss).
+        inv IN. eapply write_disjoint; eauto.
+      - exploit RELS; eauto. i. des. ss.
+      - exploit RELS; eauto. i. des. ss.
+      - exploit RELS; eauto. i. des. ss.
+      - inv LOCAL0. inv STEP. ss. revert IN.
+        repeat condtac; ss; i; des; try by (exploit RELS; eauto; i; des; ss).
+        inv IN. eapply write_na_disjoint; eauto.
+      - exploit RELS; eauto. i. des. ss.
+      - exploit RELS; eauto. i. des. ss.
+      - exploit RELS; eauto. i. des. ss.
     Qed.
   End RelWrites.
 End RelWrites.
